\documentclass[a4paper]{article}
\usepackage[pdftex]{graphicx}
\usepackage[utf8]{inputenc}
\usepackage{enumerate}
\usepackage{amssymb}
\usepackage{tikz}
\usepackage{href-ul}
\hypersetup{
	colorlinks=true,
	linkcolor=blue,
	urlcolor=blue}
\usepackage{geometry}
\geometry{a4paper, top=15mm, left=15mm, right=15mm, bottom=15mm,
	headsep=10mm, footskip=12mm}

\begin{document}
	\begin{tikzpicture}(10,3)
		\draw[ultra thick](2,0) --(10,0) -- (10,1.3) --(2,1.3) -- (2,0);
		\draw[fill=black](2,0)-- (0,.6) -- (2,.6) -- (2,0);
		\node at (6,.6) {\large Solution sheet from \href{http://www.okuyakl.com}{www.okuyakl.com}};
	\end{tikzpicture}
	\vspace{0.5 cm}
	
	\noindent{\bf Task 1.}\\
	\renewcommand{\arraystretch}{2}
	\begin{tabular}{p{8 cm}p{8 cm}}
		a) $f'(x)=2x(x-2)+(x^2+1) $ & b) $f'(x)=(3x^2-2)\sqrt{x}+(x^ 3-2x)\cdot {1\over 2}x^{-{1\over 2}} $ \\
		c) $f'(x)={1\over 2}x^{-{1\over 2}}\cdot 3x^5 + (\sqrt{x}-1)\cdot 15x^4 $ & d) $f'(x)=(2x^3+{1\over 2}x^2)(tx-7)+({1\over 2}x^4+{1\over 6}x^3)\ cdot t $\\
		e) $f'(t)=({1\over 2}t^{-{1\over 2}}+2t)t^{-1}-(t^{1\over 2}+t^2 )t^{-2} $ & f) $f'(x)=(x-b)+(x-a) $ \\
		g) $f'(x)=2t^2x(x-2t)+t^2x^2 $ & h) $f'(t)=2x^2t(x-2t)-t^2x^2\cdot2 $
	\end{tabular}
	
	\noindent{\bf Task 2.}\\
	\renewcommand{\arraystretch}{2}
	\begin{tabular}{p{4 cm}p{4 cm}p{4 cm}p{4 cm}}
		a) $f'(x)= {-2 \over x^3}$ & b) $f'(x)= {-3x^2 \over (x^3-1)^2} $ & c) $f'(x)= { 2x+1\over (x^2+x)^2} $ & d) $f'(x)= {-2(2x-2) \over (x^2-2x )^2} $ \\
		e) $f'(x)= {-21tx^2 \over (tx^3-t)^2}$ & f) $f'(t)= {-x^3+1 \over (tx^3 -t)^2}$ & g) $f'(x)= {-ab \over (bx+c)^2}$ & h) $f'(t)={6t^2+12t \over ( t^3-3t)^2} $\\
	\end{tabular}
	
	\noindent{\bf Task 3.}\\
	\renewcommand{\arraystretch}{2}
	\begin{tabular}{p{4 cm}p{4 cm}p{4 cm}p{4 cm}}
		a) $f'(x)= {1 \over (x+1)^2}$ & b) $f'(x)= {-x^2+4x \over (x-2)^2}$ & c) $f'(x)={ad-bc \over (cx+d)^2} $ & d) $f'(t)={-t^3-2t-2 \over 4t^3} $\\
		e) $f'(x)= { t^3\over (x+t)^2}$ & f) $f'(t)= { t^2x+2x^2\over (x+t)^ 2}$ & g) $f'(x)= {x^2-8x-4 \over (x-4)^2}$& h) $f'(t)= {-6t^4-12t^ 3 \over (t+1)^3}$\\
	\end{tabular}
	
	\begin{center}
		\includegraphics[width=7 cm]{../../viecher/eendcomic.pdf}
		
		Here you can go back to the \href{https://www.okuyakl.de/math/m11prqL098/ae098.pdf}{task sheet}
	\end{center}
	
\end{document}