\documentclass[a4paper]{article}
\usepackage[pdftex]{graphics}
\usepackage[utf8]{inputenc}
\usepackage{enumerate}
\usepackage{amssymb}
\usepackage{icomma}
\usepackage{tikz}
\usepackage{href-ul}
\hypersetup{
	colorlinks=true,
	linkcolor=blue,
	urlcolor=blue}
\usepackage{geometry}
\geometry{a4paper, top=15mm, left=15mm, right=15mm, bottom=15mm,
	headsep=10mm, footskip=12mm}

\begin{document}
	\begin{tikzpicture}(10,3)
		\draw[ultra thick](2,0) --(10,0) -- (10,1.3) --(2,1.3) -- (2,0);
		\draw[fill=black](2,0)-- (0,.6) -- (2,.6) -- (2,0);
		\node at (6,.6) {\large solution sheet from \href{http://www.okuyakl.com}{www.okuyakl.com}};
	\end{tikzpicture}
	\vspace{0.5 cm}
	
	\noindent{\bf Task 1.}\\
	\begin{minipage}{0.5\textwidth}
		\includegraphics[width=7 cm]{gbrf049}
	\end{minipage}
	\hfill
	\begin{minipage}{0.5\textwidth}
		$$
		\begin{array}{rcll}
			{1 \over x-2} - 1 &=& 0 & | +1\\
			{1 \over x-2} &=& 1 & | \cdot (x-2)\\
			1 &=&(x-2 \\|+2\\
			3 &=& x
		\end{array}
		$$
		The zero is at $N(3|0)$
	\end{minipage}
	
	
	\noindent {\bf task 2.}\\
	The factor $(x-2)$ also appears in the denominator $(2x-4)=2(x-2)$. So the main denominator is $2(x-4)$.
	So we just expand the second fraction with $2$ and get two fractions with the same name, which we add as follows:
	$${x \over 2(x-2)} + {2 \over 2(x-2)}= {x+2 \over 2(x-2)} $$
	We also get this result if we reduce the fraction from the problem:
	$${x^2-4\over (2x-4)(x-2)}= {(x+2)(x-2)\over 2(x-2)^2}= {x+2 \over 2(x-2)}$$
	\vspace{0.5 cm}
	
	\noindent{\bf Task 3.}\\
	
	\renewcommand{\arraystretch}{2}
	\begin{tabular}{p{3 cm}p{3 cm}p{3 cm}p{3 cm}}
		a) $x=-2$ & b) $y=4$ & c) $x=1$ & d) $x=-{1\over5}$ \\
		e) $x=2$ & f) $x=3$ & g) $x=5$ & h) $x=3$\\
		i) $x=10$ & j) $x=-18$ & k) $x=-{1\over2}$ &
	\end{tabular}
	\vspace{0.5 cm}
	
	\noindent {\bf task 3. l)}\\
	We factor both denominators:
	$$
	\renewcommand{\arraystretch}{2}
	\begin{array}{rcll}
		{1 \over 2(3x-1)} &=& 1 + {x \over 3(3x-1)} &| \cdot 6(3x-1)\\
		3 &=& 6(3x-1) + 2x \\
		3 &=& 18x-6 +2x &|+6 \\
		9 &=& 20x &|:20 \\
		0.45 &=& x
	\end{array}
	$$
	\vspace{0.5 cm}
	
	\noindent {\bf task 4.}\\
	
	\renewcommand{\arraystretch}{2}
	\begin{tabular}{p{3.5 cm}p{3.5 cm}p{3.5 cm}p{3.5 cm}}
		a) $1$ &b) $-{1\over 2x+2}$ &c) ${2\over(x+1)(x+3)}$ &d) ${2\over x+5}$ \\
		e) $x+1$ & f) ${2x+1 \over 1-x}$ &g) ${1\over 3-x}$ &h) $3x-24$ \\
		i) ${4 \over x+1}$ & j) ${-x-2 \over 2} $
	\end{tabular}
	\vspace{0.5 cm}
	
	\noindent {\bf task 4. k)}\\
	$${5x \over x-2} \cdot {-2(x-2) \over x(x+2)}=-{10 \over x+2}$$
	\vspace{0.5 cm}
	
	\noindent {\bf task 4. l)}\\
	$$\left({1 \over 2x}+{2 \over x}\right): {3 \over x-1}= {1+4 \over 2x} \cdot {x-1 \over 3} = {5(x-1) \over 6x}$$
	\vspace{0.5 cm}
	
	\noindent{\bf Task 5.}\\
	\renewcommand{\arraystretch}{2}
	\begin{tabular}{p{3 cm}p{3 cm}p{3 cm}p{3 cm}}
		a) $x$ &b) ${2\over x^2} $ &c) ${1\over 2x} $ &d) ${x^2 \over 49}$ \\
		e) ${1\over 4x+4} $ & f) ${2\over 7x} $ &g) $1 $ &h) ${t^3 \over 4} $ \\
		i) $x-1 $ & j) ${3\over 2}$ & k) ${1\over 4y-2} $ & l) ${1\over2}(x+1) $ \\
	\end{tabular}
	
	\begin{center}
		\includegraphics[width=7 cm]{../../viecher/eendcomic.pdf}
		
		Here you can go back to the \href{https://www.okuyakl.de/math/m8brtL049/ae049.pdf}{task sheet}
	\end{center}
	
\end{document}