\documentclass[a4paper]{article}
\usepackage[pdftex]{graphicx}
\usepackage[utf8]{inputenc}
\usepackage{enumerate}
\usepackage{icomma}
\usepackage{amssymb}
\usepackage{amsmath}
\usepackage{tikz}
\usepackage{href-ul}
\hypersetup{
	colorlinks=true,
	linkcolor=blue,
	urlcolor=blue}
\usepackage{geometry}
\geometry{a4paper, top=15mm, left=15mm, right=15mm, bottom=15mm,
	headsep=10mm, footskip=12mm}

\begin{document}
	\begin{tikzpicture}(10,3)
		\draw[ultra thick](2,0) --(10,0) -- (10,1.3) --(2,1.3) -- (2,0);
		\draw[fill=black](2,0)-- (0,.6) -- (2,.6) -- (2,0);
		\node at (6,.6) {\large Solution sheet from \href{http://www.okuyakl.com}{www.okuyakl.com}};
	\end{tikzpicture}
	\vspace{0.5 cm}
	
	\noindent{\bf Task 1. a)}\\
	We can immediately specify the function term:
	$$f^*(x)=0.25x^{-5}$$
	\noindent{\bf Task 1. b)}\\
	Set of definitions and values:
	$$\mathbb{D}= \mathbb{R} \setminus \{0\} \qquad \mathbb{W}= \mathbb{R} \setminus \{0\} $$
	Asymptotes are $x=0$ and $y=0$.
	Symmetry:
	$$f^*(-x)=0.25(-x)^{-5} = -0.25x^{-5}=-f^*(x) $$
	The new function is point symmetric.
	
	\noindent{\bf Task 1. c)}\\
	$$
	\renewcommand{\arraystretch}{2}
	\begin{array}{rccl}
		& x'&=& x+3 \\
		\land & y' &=& y+4 \\
		\hline
		& x&=& x'-3 \\
		\land & y' &=& 0.25x^{-5}+4\\
		\hline
		\Rightarrow & y' &=& 0.25(x'-3)^{-5}+4\\
		& f^{**}(x)&=& 0.25(x-3)^{-5}+4
	\end{array}
	$$
	\begin{minipage}{0.5\textwidth}
		\noindent{\bf Task 2. a)}\\
		$$f_2(x)=0.5x^4$$
		$$f_3(x)=0.5(x-4)^4+1$$
		\noindent{\bf Task 2. b)}\\
		$$\mathbb{D}_{f_3}=\mathbb{R}$$
		$$\mathbb{W}_{f_3}=[1;\infty[$$
	\end{minipage}
	\hfill
	\begin{minipage}{0.5\textwidth}
		\includegraphics[width=7 cm]{otto208}
	\end{minipage}
	
	\noindent{\bf Task 3. a)}\\
	$$\mathbb{D}_{f}=\mathbb{R}\setminus \{1\}$$
	$$\mathbb{W}_{f}=[3;\infty[$$
	Since the set of values only includes positive numbers, the graph never intersects the x-axis.
	\vspace{0.5 cm}
	
	\begin{minipage}{0.5\textwidth}
		\noindent{\bf Task 3. b) c) and d)}\\
		$$
		\renewcommand{\arraystretch}{2}
		\begin{array}{rccl}
			& x'&=& x-3 \\
			\land & y' &=& y-4 \\
			\hline
			& x&=& x'+3 \\
			\land & y' &=& 2(x-1)^{-2}+3-4\\
			\hline
			\Rightarrow & y' &=& 2(x'+3-1)^{-2}-1\\
			& h(x)&=& 2(x+2)^{-2}-1
		\end{array}
		$$
	\end{minipage}
	\hfill
	\begin{minipage}{0.5\textwidth}
		\includegraphics[width=7 cm]{holl208}
	\end{minipage}
	
	\noindent{\bf Task 3. e)}\\
	The horizontal asymptote is at $y=-1$; the vertical is at $x=-2$.
	
	\noindent{\bf Task 3. f)}\\
	According to the instructions we show:
	$$f(-2+a)=2(-2+a+2)^{-2}-1 = 2a^{-2}-1$$
	$$f(-2-a)=2(-2-a+2)^{-2}-1 = 2(-a)^{-2}-1 =2a^{-2}-1=f (-2+a) $$
	The line $x=-2$ is the axis of symmetry.
	
	\noindent{\bf Task 3. g)}\\
	$$
	\renewcommand{\arraystretch}{2}
	\begin{array}{rcll}
		2(x+2)^{-2}-1 &=& 0 &|+1\\
		{2 \over (x+2)^2} &=& 1 &|\cdot (x+2)^2\\
		2 &=& (x+2)^2 &|\pm \sqrt{\quad}\\
		\pm \sqrt{2} &=& x+2 &|-2\\
		\pm\sqrt{2}-2 &=& x \\
		x_1 &=& \sqrt{2}-2 \\
		x_2 &=& -\sqrt{2}-2
	\end{array}
	$$
	The calculated zero points correspond to those in the diagram.
	
	\noindent{\bf Task 4.}\\
	a) $$(2+2,3)^0=1 $$
	b) $$1+\left({1\over 3}\right)^{-2}=1+3^2 = 10 $$
	c) $$1:4^{-2}=1\cdot 4^2=16$$
	d) $$2^{x+2}\cdot\left({1\over 2}\right)^{x+2} = 2^{x+2} \cdot 2^{-(x+2)} =2^0=1$$
	e) $$\left({ 2 \over a}\right)^3 \cdot (-a)^3=-2^3 =-8$$
	
	\begin{center}
		\includegraphics[width=7 cm]{../../viecher/eendcomic.pdf}
		
		Here you can go back to the \href{https://www.okuyakl.de/math/m10pofuL208/ae208.pdf}{task sheet}
	\end{center}
	
\end{document}