\documentclass[a4paper]{article}
\usepackage[pdftex]{graphicx}
\usepackage[utf8]{inputenc}
\usepackage{enumerate}
\usepackage{amssymb}
\usepackage{tikz}
\usepackage{href-ul}
\hypersetup{
	colorlinks=true,
	linkcolor=blue,
	urlcolor=blue}
\usepackage{geometry}
\geometry{a4paper, top=15mm, left=15mm, right=15mm, bottom=15mm,
	headsep=10mm, footskip=12mm}

\begin{document}
	
\begin{tikzpicture}(10,3)
	\draw[ultra thick](2,0) --(10,0) -- (10,1.3) --(2,1.3) -- (2,0);
	\draw[fill=black](2,0)-- (0,.6) -- (2,.6) -- (2,0);
	\node at (6,.6) {\large Lösungsblatt von \href{https://www.okuyakl.de}{www.okuyakl.de}};
\end{tikzpicture}
\vspace{0.5 cm}

	\noindent{\bf Aufgabe 1.}\\
	\renewcommand{\arraystretch}{3}
	\begin{tabular}{p{8 cm}p{8 cm}}
		a) $f'(x)=7(x^2-1)^6\cdot 2x $ & b) $f'(x)=(2x^3-x)(6x-1) $ \\ 
		c) $f'(x)=3(t^2x-4x)^2(t^2-4) $ & d) $f(t)=3(t^2x-4x)^2\cdot 2tx $\\
	\end{tabular}
	
	\noindent{\bf Aufgabe 2.}\\
	\begin{tabular}{p{8 cm}p{8 cm}}
		a) $f'(x)=2\cos 2x $ & b) $f'(x)=-\sin(x^2-1)\cdot 2x$\\
		c) $f'(x)=9\sin{x}\cdot \cos{x}$ & d) $f'(x)=-2\sin(4x-\pi)$\\
	\end{tabular}
	
	\noindent{\bf Aufgabe 3.}\\
	\begin{tabular}{p{8 cm}p{8 cm}}
		a) $f'(x)= -6e^{-3x}$ & b) $f'(x)=-2x\cdot e^{-x^2+1} $ \\
		c) $f'(x)=-{1\over x^2} \cdot e^{1\over x} $ & d) $f'(x)=a\cdot e^{ax+b} $\\
	\end{tabular}

	\noindent{\bf Aufgabe 4.}\\
	\begin{tabular}{p{8 cm}p{8 cm}}
		a) $f'(x)=2(\ln(x)-1)\cdot {1\over x}$ & b) $f'(x)=-{1\over x}$ \\
		c) $f'(t)={2x\over 2tx +5 }$ & d) $f'(x)={2ax+b \over ax^2+bx+c}$\\
	\end{tabular}

	
	\noindent{\bf Aufgabe 5.}\\
	\begin{tabular}{p{8 cm}p{8 cm}}
		a) $f'(x)=(2x-1)^{-{1\over 2}} $ & b) $f'(x)={1\over 2}(t^2x^3+2t)^{-{1\over 2}}\cdot 3t^2x^2 $ \\
		c) $f'(t)={1\over 2}({t^2x^3+2t})^{-{1\over 2}}\cdot(2tx^3+2) $ & d) $f'(x)={3\over 2}(7x+1)^{1\over 2}\cdot 7 $\\
	\end{tabular}
	
	\noindent{\bf Aufgabe 6.}\\
	a)$\tan{x}={\sin x \over \cos x}$:
	$$f'(x)={1 \over (\cos x)^2}$$
	b)$(u(v(w(x))))'=u'(v(w(x)))\cdot v'(w(x)) \cdot w'(x)$:
	$$f'(x)=7(\sin(2x))^6 \cdot \cos(2x) \cdot 2$$
	c)$x^x=e^{x\cdot \ln x}$:
	$$f'(x)=(\ln x + 1) \cdot e^{x\cdot \ln x}$$
	

\begin{center}
	\includegraphics[width=7 cm]{../../viecher/endcomic.pdf}
	
	Hier geht es zurück zum \href{https://www.okuyakl.de/math/m11kerL097/aa097.pdf}{Aufgabenblatt}
\end{center}

\end{document}

