\documentclass[a4paper]{article}
\usepackage[pdftex]{graphicx}
\usepackage[utf8]{inputenc}
\usepackage{enumerate}
\usepackage{icomma}
\usepackage{amssymb}
\usepackage{polynom}
\usepackage{tikz}
\usepackage{href-ul}
\hypersetup{
	colorlinks=true,
	linkcolor=blue,
	urlcolor=blue}
\usepackage{geometry}
\geometry{a4paper, top=10mm, left=15mm, right=15mm, bottom=15mm,
	headsep=0mm, footskip=12mm}


\begin{document}
	\begin{tikzpicture}(10,3)
		\draw[ultra thick](2,0) --(10,0) -- (10,1.3) --(2,1.3) -- (2,0);
		\draw[fill=black](2,0)-- (0,.6) -- (2,.6) -- (2,0);
		\node at (6,.6) {\large Solution sheet from \href{http://www.okuyakl.com}{www.okuyakl.com}};
	\end{tikzpicture}
	\vspace{0.5 cm}
	
	\noindent{\bf Task 1.}\\
	a) $$(x+7)(x+11)$$
	b) $$2x^2-14x \stackrel{\rm OFF}{=} 2x(x-7)$$
	c) When factoring with the solution formula, the factor in front of the $x^2$ must be taken into account:
	$$x_{1/2}=\frac{2\pm \sqrt{4-2\cdot (-{3\over 2})}}{4} \Rightarrow \quad x_1 = -{1\over 2} ;\quad x_2={3\over 2} \Rightarrow f(x)= 2\cdot(x+{1\over 2})(x-{3\over 2})$$
	d) the polynomial division yields:
	$$
	\polyset{style=C,div=:,vars=x}
	\polylongdiv{2x^3-9x^2+7x+6}{x-3}
	$$
	We factor with the solution formula, the factor in front of $x^2$ is again $2$:
	$$ f(x)=(x-3)(2x^2-3x-2)\stackrel{\textnormal{SOL}}{=}2 \cdot (x-3)(x+0.5)(x -2)$$
	\noindent{\bf Task 2.}\\
	a) We substitute $u=x^2$ and then decompose:
	$$f(x)=u^2-13u+36 \stackrel{\textnormal{VIE}}{=}(u-4)(u-9) \Rightarrow u_1= 4;\quad u_2=9$$
	$$ \textnormal{Back substitution:}\quad x_1=2\qquad x_2=-2 \qquad x_3=3 \qquad x_4=-3$$
	$$f(x)=(x+2)(x-2)(x+3)(x-3)$$
	b) Here it makes sense to exclude it, since $x$ occurs everywhere. We then apply the solution formula:
	$$x^2(2x^2+x-10)=0 \Rightarrow x_{1/2}=0 $$
	$$ x_{3/4}=\frac{-1\pm \sqrt{1-4\cdot 2\cdot (-10)}}{2\cdot 2} \quad \Rightarrow \quad x_3=-2, 5 \quad x_4=2$$
	$$f(x)=2x^2(x+2.5)(x-2)$$
	c) The polynomial division gives:
	$$
	\polyset{style=C,div=:,vars=x}
	\polylongdiv{x^3+x^2-102x+360}{x+12}
	$$
	Now Vieta's theorem comes into play:
	$$f(x)=(x+12)(x^2-11x+30)=(x+12)(x-5)(x-6)$$
	d) first we exclude $x^2$ and get:
	$$f(x)=x^2\cdot(5x^4-30x^2-275)=0 \qquad x_{1/2}=0$$
	in the second term we substitute $u=x^2$:
	$$5u^2-30u-275=0 \qquad | :5$$
	Now we can solve this quadratic equation (SOL; VIE):
	$$u^2- 6u - 55= 0 =(u-11)\cdot(u+5)$$
	Back substitution provides:
	$$x^2=11 \Rightarrow x_3=\sqrt{11}\, ; \quad x_4=-\sqrt{11}$$
	
	$$x^2=-5 \quad \textnormal{no further solution}$$
	e) First we exclude $x$:
	$$x\cdot(x^4+6x^3+5x^3-24x-36)=0\,;\quad x_1=0$$
	Then we subject the term to two polynomial divisions:
	$$
	\polyset{style=C,div=:,vars=x}
	\polylongdiv{x^4+6x^3+5x^2-24x-36}{x-2}
	$$
	$$
	\polyset{style=C,div=:,vars=x}
	\polylongdiv{x^3+8x^2+21x+18}{x+2}
	$$
	The obtained term is reminiscent of a binomial formula:
	$$x^2+6x+9=(x+3)^2$$
	So the further solutions are:$$x_{4/5}=-3$$
	
	\begin{center}
		\includegraphics[width=7 cm]{../../viecher/eendcomic.pdf}
		
		Here you can go back to the \href{https://www.okuyakl.de/math/m11nstL174/ae174.pdf}{task sheet}
	\end{center}
	
\end{document}