\documentclass[a4paper]{article}
\usepackage[pdftex]{graphicx}
\usepackage[utf8]{inputenc}
\usepackage{enumerate}
\usepackage{icomma}
\usepackage{amssymb}
\usepackage{tikz}
\usepackage{href-ul}
\hypersetup{
	colorlinks=true,
	linkcolor=blue,
	urlcolor=blue}
\usepackage{geometry}
\geometry{a4paper, top=15mm, left=15mm, right=15mm, bottom=15mm,
	headsep=10mm, footskip=12mm}

\begin{document}
	\begin{tikzpicture}(10,3)
		\draw[ultra thick](2,0) --(10,0) -- (10,1.3) --(2,1.3) -- (2,0);
		\draw[fill=black](2,0)-- (0,.6) -- (2,.6) -- (2,0);
		\node at (6,.6) {\large Solution sheet from \href{http://www.okuyakl.com}{www.okuyakl.com}};
	\end{tikzpicture}
	\vspace{0.5 cm}
	
	\noindent{\bf Task 1.}\\
	This figure describes a rotation around the origin by $\sin^{-1}0.80 = 53.1^\circ$.
	
	\noindent{\bf Task 2.}\\
	We compare with the mirror matrix from the formula collection:
	$$-0.71 = \cos 2\alpha \quad \Rightarrow \quad \alpha = {1 \over 2} \cdot \cos^{-1} (-0.71) =67.6^\circ$$
	Then follows:
	$$z=0.71 \quad y= -0.71$$
	The mirror axis has the gradient:
	$$m= \tan \alpha = \tan 67.6^\circ = 2.4 $$
	So the mirror axis is:
	$$g:\quad y=2.4x$$
	
	\noindent{\bf Task 3.}\\
	The slope angle of the line is:
	$$\alpha = \tan^{-1}\left(-{2 \over 3 }\right) =-33.7^\circ$$
	We apply the mirror matrix to the line h:
	$$ \left(
	\begin{array}{c}
		x'\\
		y'
	\end{array}
	\right) =
	\left(
	\begin{array}{cc}
		\cos 2 \alpha & \sin 2 \alpha \\
		\sin 2 \alpha & -\cos 2 \alpha
	\end{array}
	\right)
	\odot
	\left(
	\begin{array}{c}
		x\\
		y
	\end{array}
	\right)$$
	
	$$ \left(
	\begin{array}{c}
		x'\\
		y'
	\end{array}
	\right) =
	\left(
	\begin{array}{cc}
		0.385 & -0.923 \\
		-0.923 & -0.385
	\end{array}
	\right)
	\odot
	\left(
	\begin{array}{c}
		x\\
		2x +2
	\end{array}
	\right)$$
	
	$$ \left(
	\begin{array}{c}
		x'\\
		y'
	\end{array}
	\right) =
	\left(
	\begin{array}{cc}
		0.385x -1.846x -1.846\\
		-0.923x - 0.770x-0.770 \\
		
	\end{array}
	\right) =
	\left(
	\begin{array}{cc}
		-1.461x -1.846\\
		-1.693x -0.77 \\
	\end{array}
	\right)$$
	
	$$
	\renewcommand{\arraystretch}{2}
	\begin{array}{rcll}
		x &=& - 0.684 x' - 1.264 \\
		y' &=& 1.16x + 2.14 -0.77 &= 1.16x +1.37
	\end{array}
	$$
	This means $$h': y=1.16x+1.37$$
	
	
	\noindent
	\begin{minipage}{0.5\textwidth}
		\noindent{\bf Task 4. a)}\\
		\includegraphics[width=7 cm]{pasch028}
	\end{minipage}
	\hfill
	\begin{minipage}{0.5\textwidth}
		\noindent{\bf Task 4. b)}\\
		We substitute (-x) into the function term and get:
		$$f(-x)= (-x)^2 - 2\cdot (-x) +4 = x^2 +2x+4$$
		
		\noindent{\bf Task 4. c)}\\
		We form the inverse function:
		$$
		\renewcommand{\arraystretch}{2}
		\begin{array}{rcll}
			x &=& y^2+2x+4 \\
			x &=& (y+1)^2 +3 \\
			x-3 &=& (y+1)^2 \\
			\sqrt{x-3} &=& y+1 \\
			\sqrt{x-3}-1 &=& y
		\end{array}
		$$
	\end{minipage}
	
	\begin{center}
		\includegraphics[width=7 cm]{../../viecher/eendcomic.pdf}
		
		Here you can go back to the \href{https://www.okuyakl.de/math/m10rsabbL028/ae028.pdf}{task sheet}
	\end{center}
	
\end{document}